src/FcEtt/dep_prog.v
@@ -20,7 +20,7 @@ Notation "!!"          := (inright _ _).
 
 
 Hint Resolve inleft inright left right.
-
+(*
 (* Notations: _ <- _; _ is the notation for destructing a sumor, >--> for destructing a sumbool.
    Notation convention: the arrows are 1 dash longer when the return (type) constructor is different, e.g. destructing a sumbool to return a sumor. *)
 Notation "x <- e1 ; e2" :=
@@ -72,3 +72,4 @@ Notation "e1 >---> e2" :=
      | left _ => e2
    end)
 (right associativity, at level 60).
+*)
